Phi_System/IDE_CP_App2.thy
@@ -87,6 +87,38 @@ lemma [\<phi>reason %To_ToA_fallback]:
   unfolding Action_Tag_def Transformation_def
   by clarsimp
 
+subsubsection \<open>Short-cut of ToA\<close>
+
+text \<open>We can assume the name bindings of values are lambda-equivalent. \<close>
+
+\<phi>reasoner_group Val_ToA = (1100, [1100, 1120]) in ToA_cut
+  \<open>Short-cut transformations about values\<close>
+
+lemma [\<phi>reason %Val_ToA+20 for \<open>_ \<heavy_comma> _ \<Ztypecolon> \<v>\<a>\<l>[_] _ \<t>\<r>\<a>\<n>\<s>\<f>\<o>\<r>\<m>\<s> _ \<Ztypecolon> \<v>\<a>\<l>[_] _ \<r>\<e>\<m>\<a>\<i>\<n>\<s>[_] _ \<w>\<i>\<t>\<h> _\<close>]:
+  "R \<heavy_comma> x \<Ztypecolon> \<v>\<a>\<l>[v] T \<t>\<r>\<a>\<n>\<s>\<f>\<o>\<r>\<m>\<s> x \<Ztypecolon> \<v>\<a>\<l>[v] T \<r>\<e>\<m>\<a>\<i>\<n>\<s>[True] R"
+  unfolding REMAINS_def Transformation_def by simp
+
+lemma [\<phi>reason %Val_ToA+10 for \<open>_ \<heavy_comma> _ \<Ztypecolon> \<v>\<a>\<l>[_] _ \<t>\<r>\<a>\<n>\<s>\<f>\<o>\<r>\<m>\<s> _ \<Ztypecolon> \<v>\<a>\<l>[_] _ \<r>\<e>\<m>\<a>\<i>\<n>\<s>[_] _ \<w>\<i>\<t>\<h> _\<close>
+                    if \<open>PLPR_Env.boolean_flag \<^const_name>\<open>ToA_flag_deep\<close> true o Context.Proof o fst\<close>]:
+  " y \<Ztypecolon> U \<t>\<r>\<a>\<n>\<s>\<f>\<o>\<r>\<m>\<s> x \<Ztypecolon> T \<w>\<i>\<t>\<h> P
+\<Longrightarrow> R \<heavy_comma> y \<Ztypecolon> \<v>\<a>\<l>[v] U \<t>\<r>\<a>\<n>\<s>\<f>\<o>\<r>\<m>\<s> x \<Ztypecolon> \<v>\<a>\<l>[v] T \<r>\<e>\<m>\<a>\<i>\<n>\<s>[True] R \<w>\<i>\<t>\<h> P"
+  unfolding Transformation_def
+  by (simp add: times_list_def) metis
+
+lemma [\<phi>reason %Val_ToA]:
+  " R \<t>\<r>\<a>\<n>\<s>\<f>\<o>\<r>\<m>\<s> x \<Ztypecolon> \<v>\<a>\<l>[v] T \<r>\<e>\<m>\<a>\<i>\<n>\<s>[True] R' \<w>\<i>\<t>\<h> P
+\<Longrightarrow> R \<heavy_comma> X \<t>\<r>\<a>\<n>\<s>\<f>\<o>\<r>\<m>\<s> x \<Ztypecolon> \<v>\<a>\<l>[v] T \<r>\<e>\<m>\<a>\<i>\<n>\<s>[True] R'\<heavy_comma> X \<w>\<i>\<t>\<h> P"
+  unfolding REMAINS_def split_paired_All
+  by (simp; metis transformation_left_frame mult.assoc mult.commute)
+
+lemma [\<phi>reason %Val_ToA except \<open>_ \<t>\<r>\<a>\<n>\<s>\<f>\<o>\<r>\<m>\<s> ?x \<Ztypecolon> \<v>\<a>\<l>[?v] ?V \<r>\<e>\<m>\<a>\<i>\<n>\<s>[_] _ \<w>\<i>\<t>\<h> _\<close>]:
+  " R \<t>\<r>\<a>\<n>\<s>\<f>\<o>\<r>\<m>\<s> X \<r>\<e>\<m>\<a>\<i>\<n>\<s>[True] R' \<w>\<i>\<t>\<h> P
+\<Longrightarrow> R \<heavy_comma> x \<Ztypecolon> \<v>\<a>\<l>[v] V \<t>\<r>\<a>\<n>\<s>\<f>\<o>\<r>\<m>\<s> X \<r>\<e>\<m>\<a>\<i>\<n>\<s>[True] R' \<heavy_comma> x \<Ztypecolon> \<v>\<a>\<l>[v] V \<w>\<i>\<t>\<h> P"
+  unfolding REMAINS_def
+  by (metis (no_types, opaque_lifting) transformation_right_frame mult.assoc mult.commute)
+
+
+
 
 subsection \<open>Access of Local Values\<close>
 
