Phi_System/IDE_CP_Reasoning2.thy
@@ -10,31 +10,8 @@ subsection \<open>For Specific \<phi>-Types\<close>
 
 subsubsection \<open>Value\<close>
 
-text \<open>The rules require the same values are alpha-beta-eta-conversible. \<close>
+
 text \<open>Priority shouldn't exceed 2000.\<close>
-
-lemma [\<phi>reason 1215 for \<open>_ \<heavy_comma> _ \<Ztypecolon> \<v>\<a>\<l>[_] _ \<t>\<r>\<a>\<n>\<s>\<f>\<o>\<r>\<m>\<s> _ \<Ztypecolon> \<v>\<a>\<l>[_] _ \<r>\<e>\<m>\<a>\<i>\<n>\<s>[_] _ \<w>\<i>\<t>\<h> _\<close>]:
-  "R \<heavy_comma> x \<Ztypecolon> \<v>\<a>\<l>[v] T \<t>\<r>\<a>\<n>\<s>\<f>\<o>\<r>\<m>\<s> x \<Ztypecolon> \<v>\<a>\<l>[v] T \<r>\<e>\<m>\<a>\<i>\<n>\<s>[True] R"
-  unfolding REMAINS_def Transformation_def by simp
-
-lemma [\<phi>reason 1210 for \<open>_ \<heavy_comma> _ \<Ztypecolon> \<v>\<a>\<l>[_] _ \<t>\<r>\<a>\<n>\<s>\<f>\<o>\<r>\<m>\<s> _ \<Ztypecolon> \<v>\<a>\<l>[_] _ \<r>\<e>\<m>\<a>\<i>\<n>\<s>[_] _ \<w>\<i>\<t>\<h> _\<close>
-                    if \<open>PLPR_Env.boolean_flag \<^const_name>\<open>ToA_flag_deep\<close> true o Context.Proof o fst\<close>]:
-  " y \<Ztypecolon> U \<t>\<r>\<a>\<n>\<s>\<f>\<o>\<r>\<m>\<s> x \<Ztypecolon> T \<w>\<i>\<t>\<h> P
-\<Longrightarrow> R \<heavy_comma> y \<Ztypecolon> \<v>\<a>\<l>[v] U \<t>\<r>\<a>\<n>\<s>\<f>\<o>\<r>\<m>\<s> x \<Ztypecolon> \<v>\<a>\<l>[v] T \<r>\<e>\<m>\<a>\<i>\<n>\<s>[True] R \<w>\<i>\<t>\<h> P"
-  unfolding Transformation_def
-  by (simp add: Val_expn times_list_def) metis
-
-lemma [\<phi>reason 1200]:
-  " R \<t>\<r>\<a>\<n>\<s>\<f>\<o>\<r>\<m>\<s> x \<Ztypecolon> \<v>\<a>\<l>[v] T \<r>\<e>\<m>\<a>\<i>\<n>\<s>[True] R' \<w>\<i>\<t>\<h> P
-\<Longrightarrow> R \<heavy_comma> X \<t>\<r>\<a>\<n>\<s>\<f>\<o>\<r>\<m>\<s> x \<Ztypecolon> \<v>\<a>\<l>[v] T \<r>\<e>\<m>\<a>\<i>\<n>\<s>[True] R'\<heavy_comma> X \<w>\<i>\<t>\<h> P"
-  unfolding REMAINS_def split_paired_All
-  by (simp; metis transformation_left_frame mult.assoc mult.commute)
-
-lemma [\<phi>reason 1200 except \<open>_ \<t>\<r>\<a>\<n>\<s>\<f>\<o>\<r>\<m>\<s> ?x \<Ztypecolon> \<v>\<a>\<l>[?v] ?V \<r>\<e>\<m>\<a>\<i>\<n>\<s>[_] _ \<w>\<i>\<t>\<h> _\<close>]:
-  " R \<t>\<r>\<a>\<n>\<s>\<f>\<o>\<r>\<m>\<s> X \<r>\<e>\<m>\<a>\<i>\<n>\<s>[True] R' \<w>\<i>\<t>\<h> P
-\<Longrightarrow> R \<heavy_comma> x \<Ztypecolon> \<v>\<a>\<l>[v] V \<t>\<r>\<a>\<n>\<s>\<f>\<o>\<r>\<m>\<s> X \<r>\<e>\<m>\<a>\<i>\<n>\<s>[True] R' \<heavy_comma> x \<Ztypecolon> \<v>\<a>\<l>[v] V \<w>\<i>\<t>\<h> P"
-  unfolding REMAINS_def
-  by (metis (no_types, opaque_lifting) transformation_right_frame mult.assoc mult.commute)
 
 
 (*DO NOT REMOVE, for Auto_Transform_Hint
