Phi_System/IDE_CP_Reasoning3.thy
@@ -5,7 +5,7 @@ the previous part I.\<close>
 
 
 theory IDE_CP_Reasoning3
-  imports Phi_Types
+  imports IDE_CP_App2
 begin
 
 
@@ -549,6 +549,7 @@ let_\<phi>type \<phi>MapAt   deriving \<open>Gen_Br_Join ((\<^bold>\<rightarrow>
 let_\<phi>type \<phi>MapAt_L deriving \<open>Gen_Br_Join ((\<^bold>\<rightarrow>\<^sub>@) k) ((\<^bold>\<rightarrow>\<^sub>@) k') ((\<^bold>\<rightarrow>\<^sub>@) k) P (k' = k)\<close>
 let_\<phi>type \<phi>Share   deriving \<open>Gen_Br_Join ((\<odiv>) n) ((\<odiv>) m) ((\<odiv>) (If P n m)) P True\<close>
 let_\<phi>type Nosep    deriving \<open>Gen_Br_Join Nosep Nosep Nosep P True\<close>
+let_\<phi>type Val      deriving \<open>Gen_Br_Join (Val v) (Val v) (Val v) P True\<close>
 
 (*TODO: improve simplification*)
 
